Fstar/fun/Implmenetations/Utils.Heap.fst
@@ -58,3 +58,4 @@ let lookup #_ {maps_to} val' = Map.select val' maps_to
 
 val size (#a : Type) : t a -> int
 let size #a = Mkt?.size
+
